\chapter{Reconciling the Two Semantics}
In this chapter, we look at several attempts to connect the recurrences described in chapters 2 and 3. We will offer
several methods of translating from one expression language to the other, and investigate the validity of these approaches.

As a first attempt, we consider a simple recurrence with an initial condition
\begin{align*}
T(1) &= 0 \\
T(n) &= 1 + T(n/2 ) 
\end{align*}
As in the example in chapter 3, we assume that the domain of $T$ is positive powers of $2$.

This is the kind of recurrence described in chapter 3. In order to make this fit the definition of a recurrence described in 
chapter 2 --- that is, a recurrence of the form $T(n) = a(n) + T(m(n))$, we may interpret $a$ as a 
piecewise function with two sub-functions: one for the general recurrence and one for the initial condition.
We can instead write this as a single recurrence
\begin{align*}
T(n) &= a(n) + T(m(n)) \\
m(n) &= n/2, \ \forall n \\ 
a(n) &=
\begin{cases} 
0, \ n \leq 1 \\
1, \ n > 1
\end{cases}
\end{align*} 
This recurrence can then by expressed in our chapter 2 syntax as 
\begin{align*}
\texttt{T} &= \texttt{rec}(a,m) \\
m &= \lambda x.x/\texttt{2} \\
a &= \lambda x.\ifelse{x\leq\texttt{1}}{\texttt{0}}{\texttt{1}} \\
\llbracket \texttt{T} \rrbracket(d) &= \llbracket \texttt{rec}(a,m) \rrbracket(d) \\
&= \sum_{i=0}^{\infty}\llbracket a \rrbracket(\llbracket m\rrbracket^i(d)) \\
&= \sum_{i=0}^{\log(n)-1} 1 + \sum_{i=log(n)}^{\infty} 0 \\
&= \log(n) - 1
\end{align*}

However, this approach will not work in every case. Let us try to use the same process on the following recurrence
\begin{align*}
T(1) &= 1 \\
T(n) &= 2 + T(n/2) 
\end{align*}
We first write this as a single recurrence. See that, unlike the previous example, $a$ never maps to $0$.
\begin{align*}
T(n) &= a(n) + T(m(n)) \\
m(n) &= n/2, \ \forall n \\ 
a(n) &= 
\begin{cases}
1, \ n \leq 1 \\
2, \ n > 1
\end{cases}
\end{align*}
We then express this recurrence using our chapter 2 syntax as
\begin{align*}
\texttt{T} &= \texttt{rec}(a,m) \\
m &= \lambda x.x/\texttt{2} \\
a &=\lambda x.\ifelse{x\leq\texttt{1}}{\texttt{1}}{\texttt{2}} \\
\llbracket \texttt{T} \rrbracket(d) &= \llbracket \texttt{rec}(a,m) \rrbracket(d) \\
&= \sum_{i=0}^{\infty}\llbracket a \rrbracket(\llbracket m\rrbracket^i(d)) \\
&= \sum_{i=0}^{\log(n)-1} 2 + \sum_{i=\log(n) }^{\infty} 1 \\
&= \infty
\end{align*}
Which, clearly, is not a correct solution to this recurrence.

A second attempt takes a similar approach to writing a recurrence with an initial condition as a recurrence of 
the form $T(n) = a(n) + T(m(n))$. Suppose that we interpret $a$ as a piecewise function with three sub-functions:
one for the general recurrence, one for the initial condition, and one for values smaller than the initial condition, which all
map to $0$. Considering the example that failed in the previous attempt, we would have
\begin{align*}
T(n) &= a(n) + T(m(n)) \\
m &= n/2, \forall n \\
a(n) &=
\begin{cases}
0, \ n < 1 \\
1, \ n = 1 \\
2, \ n > 1
\end{cases} \\
\end{align*}
We can express this recurrence using our fixed-point syntax as
\begin{align*}
\texttt{T} &= \texttt{rec}(a,m) \\
m &= \lambda x.x/\texttt{2} \\
a &= \lambda x.\ifelse{x <1}{0}{(\ifelse{x = 1}{1}{2})} \\
\llbracket a \rrbracket(d) &= 
 \begin{cases}
0, \ d < 1 \\
1, \ d = 1 \\
2, \ d > 1 
\end{cases} \\
\llbracket \texttt{T} \rrbracket(d) &= \llbracket \texttt{rec}(a,m)\rrbracket(d) \\
&= \sum_{i=0}^{\infty}\llbracket a \rrbracket(\llbracket m\rrbracket^i(d)) \\
&= \sum_{i=0}^{\log(n)-1} 2 + \sum_{i=\log(n) }^{\log(n)} 1 + \sum_{i = \log(n) + 1}^{\infty} 0 \\
&= 2\log(n) - 1
\end{align*}

This approach matches our intuition for how an initial condition should work---that once you reach the initial condition,
you stop recursing. 

With this in mind, we can identify a general strategy for extracting a recurrence in our chapter 2 syntax (with
the $\texttt{rec}$ operator),given a recurrence in our chapter 3 syntax (with the $\texttt{fix}$ operator). 
While we cannot extract a recurrence from every $\texttt{fix}(\lambda f \lambda x.e)$ expression, we can achieve this
if $e$ is of a form that corresponds to a recurrence with an initial condition. 

Suppose we have a recurrence with an initial condition, given as follows:
\begin{align*}
T(b) &= c, \text{ where } b, \ c, \ \in \R \\
T(x) &= a(x) + T(m(x)).
\end{align*}
We write this recurrence in our chapter 3 syntax as 
\begin{align*}
\texttt{fix}(\lambda f.\lambda x. \ifelse{x = m}{c}{a(x) + f(m(x))}),
\end{align*}
an expression whose denotation will be a function $F$ such that
\begin{align*}
F(x) &=
\begin{cases}
c \text{ if } x = b \\
a(x) + c \text{ if } m(x) = b \\
a(x) + a(m(x)) + c \text{ if } m(m(x)) = b \\
\ldots \\
\sum_{i=1}^{n} a(m^{i-1}(x)) + c \text{ if } m^n(x) = b
\end{cases}
\end{align*}

We may then write this recurrence in our chapter 2 syntax as $\texttt{rec}(a',m)$, where m is the same function
as in the previous recurrence, and
\begin{align*}
a' = \lambda x.\lambda f. \ifelse{x < b}{0}{(\ifelse{x = b}{c}{a(x)})}.
\end{align*}
Then the denotation of $\texttt{rec}(a',m)$ is a function F' such that 
\begin{align*}
F'(x) &= \sum_{i=0}^{\infty} \llbracket a' \rrbracket(\llbracket m \rrbracket^i(x)) \\
&= \sum_{i=0}^{n-1} \llbracket a' \rrbracket( \llbracket m \rrbracket^i(x)) + \sum_{i=n}^n c + \sum_{i = n+1}^{\infty} 0 \\
&\text{ where } \llbracket m \rrbracket^n(x) = b \\
&= \sum_{i=1}^{n}\llbracket a' \rrbracket ( \llbracket m \rrbracket^{i-1}(x)) + c
\end{align*}
See, then, that $F' = F$. Therefore, this confirms that, given an expression $e$ of the specific form
$e = \ifelse{x = m}{c}{a(x) + f(m(x))}$, we can extract a function a' such that 
\begin{align*}
\llbracket \texttt{fix}(\lambda f. \lambda x.e) \rrbracket = \llbracket \texttt{rec}(a',m)\rrbracket
\end{align*}





 